_build/default/minibug.ml
@@ -1,4 +1,0 @@
-open Parser
-
-let () =
-  print_endline "hello"
