minibug.ml
@@ -1,4 +1,17 @@
 open Parser
+open Solver
+
+module BF = Core.BugFinder(Solver)
 
 let () =
-  print_endline "hello"
+  let (assume, prog) = parse_file (Sys.argv.(1)) in
+  match BF.find_bugs 100000 prog assume with
+  | Timeout ->
+    Printf.eprintf "bug finding timed out!\n"
+  | Found (SureBug m) ->
+    Printf.eprintf "Found a sure bug!\n";
+    Solver.print_model m
+  | Found (UnsureBug _) ->
+    Printf.eprintf "Found a (un)sure bug!\n"
+  | NotFound ->
+    Printf.eprintf "☑️ No bugs found\n"
