solver.ml
@@ -1,10 +1,29 @@
 open Z3
 open Z3.Solver
 open Z3.Arithmetic
+open Core
+
+let hard_fail msg =
+  Printf.eprintf "[internal error] %s\n" msg;
+  exit 1
 
 module Solver = struct
   let ctx = mk_context []
-  
+
+  let decl_to_int model decl =
+    let e = Model.get_const_interp model decl in
+    Expr.(simplify (Option.get e) None |> to_string |> int_of_string)
+
+  let decl_to_ident decl =
+    FuncDecl.get_name decl
+    |> Symbol.to_string
+    |> Opal.explode
+
+  let extract_model (m : Model.model) : (Core.ident * int) list =
+    List.map (fun decl ->
+      (decl_to_ident decl, decl_to_int m decl)
+    ) (Model.get_const_decls m)
+
   let rec mk_expr (e : Core.aexpr) =
     match e with
     | Var n -> Integer.mk_const ctx (Symbol.mk_string ctx (Opal.implode n))
@@ -21,12 +40,23 @@ module Solver = struct
     | Beq (e1, e2) -> Boolean.mk_eq ctx (mk_expr e1) (mk_expr e2)
     | Bnot f -> Boolean.mk_not ctx (mk_form f)
 
-  let sat (f : Core.bexpr) =
+  let check_sat (f : Core.bexpr) =
     let slv = mk_simple_solver ctx in
     let pro = mk_form f in
     add slv [pro];
     match check slv [] with
-    | SATISFIABLE -> Some true
-    | UNSATISFIABLE -> Some false
-    | UNKNOWN -> None
+    | SATISFIABLE ->
+      begin match get_model slv with
+      | None ->
+        hard_fail "model extraction failed"
+      | Some m ->
+        SAT (extract_model m)
+      end
+    | UNSATISFIABLE -> UNSAT
+    | UNKNOWN -> TIMEOUT
+
+  let print_model (m : Core.partial_store) =
+    List.iter (fun (x, vx) ->
+      Printf.printf "%s := %d\n" (Opal.implode x) vx
+    ) m
 end
