test.ml
@@ -1,0 +1,261 @@
+
+(** val negb : bool -> bool **)
+
+let negb = function
+| true -> false
+| false -> true
+
+type comparison =
+| Eq
+| Lt
+| Gt
+
+(** val compOpp : comparison -> comparison **)
+
+let compOpp = function
+| Eq -> Eq
+| Lt -> Gt
+| Gt -> Lt
+
+type positive =
+| XI of positive
+| XO of positive
+| XH
+
+type z =
+| Z0
+| Zpos of positive
+| Zneg of positive
+
+module Pos =
+ struct
+  (** val succ : positive -> positive **)
+
+  let rec succ = function
+  | XI p -> XO (succ p)
+  | XO p -> XI p
+  | XH -> XO XH
+
+  (** val add : positive -> positive -> positive **)
+
+  let rec add x y =
+    match x with
+    | XI p ->
+      (match y with
+       | XI q -> XO (add_carry p q)
+       | XO q -> XI (add p q)
+       | XH -> XO (succ p))
+    | XO p -> (match y with
+               | XI q -> XI (add p q)
+               | XO q -> XO (add p q)
+               | XH -> XI p)
+    | XH -> (match y with
+             | XI q -> XO (succ q)
+             | XO q -> XI q
+             | XH -> XO XH)
+
+  (** val add_carry : positive -> positive -> positive **)
+
+  and add_carry x y =
+    match x with
+    | XI p ->
+      (match y with
+       | XI q -> XI (add_carry p q)
+       | XO q -> XO (add_carry p q)
+       | XH -> XI (succ p))
+    | XO p ->
+      (match y with
+       | XI q -> XO (add_carry p q)
+       | XO q -> XI (add p q)
+       | XH -> XO (succ p))
+    | XH -> (match y with
+             | XI q -> XI (succ q)
+             | XO q -> XO (succ q)
+             | XH -> XI XH)
+
+  (** val pred_double : positive -> positive **)
+
+  let rec pred_double = function
+  | XI p -> XI (XO p)
+  | XO p -> XI (pred_double p)
+  | XH -> XH
+
+  (** val compare_cont : comparison -> positive -> positive -> comparison **)
+
+  let rec compare_cont r x y =
+    match x with
+    | XI p -> (match y with
+               | XI q -> compare_cont r p q
+               | XO q -> compare_cont Gt p q
+               | XH -> Gt)
+    | XO p -> (match y with
+               | XI q -> compare_cont Lt p q
+               | XO q -> compare_cont r p q
+               | XH -> Gt)
+    | XH -> (match y with
+             | XH -> r
+             | _ -> Lt)
+
+  (** val compare : positive -> positive -> comparison **)
+
+  let compare =
+    compare_cont Eq
+
+  (** val eqb : positive -> positive -> bool **)
+
+  let rec eqb p q =
+    match p with
+    | XI p0 -> (match q with
+                | XI q0 -> eqb p0 q0
+                | _ -> false)
+    | XO p0 -> (match q with
+                | XO q0 -> eqb p0 q0
+                | _ -> false)
+    | XH -> (match q with
+             | XH -> true
+             | _ -> false)
+ end
+
+module Z =
+ struct
+  (** val double : z -> z **)
+
+  let double = function
+  | Z0 -> Z0
+  | Zpos p -> Zpos (XO p)
+  | Zneg p -> Zneg (XO p)
+
+  (** val succ_double : z -> z **)
+
+  let succ_double = function
+  | Z0 -> Zpos XH
+  | Zpos p -> Zpos (XI p)
+  | Zneg p -> Zneg (Pos.pred_double p)
+
+  (** val pred_double : z -> z **)
+
+  let pred_double = function
+  | Z0 -> Zneg XH
+  | Zpos p -> Zpos (Pos.pred_double p)
+  | Zneg p -> Zneg (XI p)
+
+  (** val pos_sub : positive -> positive -> z **)
+
+  let rec pos_sub x y =
+    match x with
+    | XI p ->
+      (match y with
+       | XI q -> double (pos_sub p q)
+       | XO q -> succ_double (pos_sub p q)
+       | XH -> Zpos (XO p))
+    | XO p ->
+      (match y with
+       | XI q -> pred_double (pos_sub p q)
+       | XO q -> double (pos_sub p q)
+       | XH -> Zpos (Pos.pred_double p))
+    | XH -> (match y with
+             | XI q -> Zneg (XO q)
+             | XO q -> Zneg (Pos.pred_double q)
+             | XH -> Z0)
+
+  (** val add : z -> z -> z **)
+
+  let add x y =
+    match x with
+    | Z0 -> y
+    | Zpos x' ->
+      (match y with
+       | Z0 -> x
+       | Zpos y' -> Zpos (Pos.add x' y')
+       | Zneg y' -> pos_sub x' y')
+    | Zneg x' ->
+      (match y with
+       | Z0 -> x
+       | Zpos y' -> pos_sub y' x'
+       | Zneg y' -> Zneg (Pos.add x' y'))
+
+  (** val opp : z -> z **)
+
+  let opp = function
+  | Z0 -> Z0
+  | Zpos x0 -> Zneg x0
+  | Zneg x0 -> Zpos x0
+
+  (** val sub : z -> z -> z **)
+
+  let sub m n =
+    add m (opp n)
+
+  (** val compare : z -> z -> comparison **)
+
+  let compare x y =
+    match x with
+    | Z0 -> (match y with
+             | Z0 -> Eq
+             | Zpos _ -> Lt
+             | Zneg _ -> Gt)
+    | Zpos x' -> (match y with
+                  | Zpos y' -> Pos.compare x' y'
+                  | _ -> Gt)
+    | Zneg x' -> (match y with
+                  | Zneg y' -> compOpp (Pos.compare x' y')
+                  | _ -> Lt)
+
+  (** val leb : z -> z -> bool **)
+
+  let leb x y =
+    match compare x y with
+    | Gt -> false
+    | _ -> true
+
+  (** val eqb : z -> z -> bool **)
+
+  let eqb x y =
+    match x with
+    | Z0 -> (match y with
+             | Z0 -> true
+             | _ -> false)
+    | Zpos p -> (match y with
+                 | Zpos q -> Pos.eqb p q
+                 | _ -> false)
+    | Zneg p -> (match y with
+                 | Zneg q -> Pos.eqb p q
+                 | _ -> false)
+ end
+
+type ident = char list
+
+type aexpr =
+| Var of ident
+| Cst of z
+| Add of aexpr * aexpr
+| Sub of aexpr * aexpr
+
+type bexpr =
+| Bcst of bool
+| Ble of aexpr * aexpr
+| Beq of aexpr * aexpr
+| Bnot of bexpr
+| Band of bexpr * bexpr
+
+module Concr =
+ struct
+  type store = ident -> z
+
+  (** val aeval : store -> aexpr -> z **)
+
+  let rec aeval s = function
+  | Var x -> s x
+  | Cst c -> c
+  | Add (e1, e2) -> Z.add (aeval s e1) (aeval s e2)
+  | Sub (e1, e2) -> Z.sub (aeval s e1) (aeval s e2)
+
+  (** val beval : store -> bexpr -> bool **)
+
+  let rec beval s = function
+  | Bcst b -> b
+  | Ble (e1, e2) -> Z.leb (aeval s e1) (aeval s e2)
+  | Beq (e1, e2) -> Z.eqb (aeval s e1) (aeval s e2)
+  | Bnot e0 -> negb (beval s e0)
+  | Band (e1, e2) -> (&&) (beval s e1) (beval s e2)
+ end
