test.mli
@@ -1,0 +1,83 @@
+
+val negb : bool -> bool
+
+type comparison =
+| Eq
+| Lt
+| Gt
+
+val compOpp : comparison -> comparison
+
+type positive =
+| XI of positive
+| XO of positive
+| XH
+
+type z =
+| Z0
+| Zpos of positive
+| Zneg of positive
+
+module Pos :
+ sig
+  val succ : positive -> positive
+
+  val add : positive -> positive -> positive
+
+  val add_carry : positive -> positive -> positive
+
+  val pred_double : positive -> positive
+
+  val compare_cont : comparison -> positive -> positive -> comparison
+
+  val compare : positive -> positive -> comparison
+
+  val eqb : positive -> positive -> bool
+ end
+
+module Z :
+ sig
+  val double : z -> z
+
+  val succ_double : z -> z
+
+  val pred_double : z -> z
+
+  val pos_sub : positive -> positive -> z
+
+  val add : z -> z -> z
+
+  val opp : z -> z
+
+  val sub : z -> z -> z
+
+  val compare : z -> z -> comparison
+
+  val leb : z -> z -> bool
+
+  val eqb : z -> z -> bool
+ end
+
+type ident = char list
+
+type aexpr =
+| Var of ident
+| Cst of z
+| Add of aexpr * aexpr
+| Sub of aexpr * aexpr
+
+type bexpr =
+| Bcst of bool
+| Ble of aexpr * aexpr
+| Beq of aexpr * aexpr
+| Bnot of bexpr
+| Band of bexpr * bexpr
+
+module Concr :
+ sig
+  type store = ident -> z
+
+  val aeval : store -> aexpr -> z
+
+  val beval : store -> bexpr -> bool
+ end
