_build/default/README.md
@@ -1,5 +1,0 @@
-# minibug
-
-Concise and documented Coq formalization of a symbolic bug finder for IMP
-
-
